Now requires Coq 8.4. Actually some files still work in 8.3; see the README. The main reason for 8.4 was function eta conversion, but this turned out not to be as helpful as I hoped. 8.4 also seems to be faster and to have slightly better type inference.
The main purpose of this revision is to update everything to support full-blown substitutions.
The previous version only allowed substituting variables, not arbitrary terms.
Thus, this upgrade paves the way for interpreting a serious dependent type theory.
(The other missing ingredient--before adding more type constructors--is interpreting judgmental equality/conversion.)

Also, the main language (in TreeSyntax.v) now has regular applications instead of argument lists.

I tried to factor out the stuff dealing only with judgment structure.
Unfortunately this makes for some pretty involved use of parameterized modules.
I wonder if it was worth it.
If only Coq had abstract base classes...

trunk/TreeSyntax.v
@@ -1,880 +1,403 @@
 Require Import List.
-Require Import Compare_dec.
+Require Import Substitutions.
+Require Import DepTyping.
 
-Require Import Utils.
-Require Import SimpSubst.
-Require Import SimpSyntax.
+Require Import Le.
 
-Require Import Le Lt.
-Require Import Plus Minus.
-Require Import Min.
+(* Tree syntax, to do typing in one context *)
+Inductive treeTerm : Set :=
+	var (i:nat) |
+	apl (f a:treeTerm).
 
-(* Tree syntax for types, to do typing in one context *)
-Inductive treeFam : Set :=
+Inductive treeType : Set :=
 	Uv |
-	El (p:nat * list nat) |
-	Pi (A B:treeFam).
+	El (t:treeTerm) |
+	Pi (A B:treeType).
 
-(* One-context substitutions *)
+Import VarBump.
 
-Definition pBump n l (p:_ * _) := let (f,la) := p in (varBump n l f,laBump n l la).
-Definition pSubst (p:_ * _) l b := let (f,la) := p in (varSubst l b f,laSubst la l b).
+Fixpoint ttBump n l t := match t with
+	var i => var (varBump n l i) |
+	apl f a => apl (ttBump n l f) (ttBump n l a)
+end.
 
-Fixpoint fBump n l F := match F with
+Fixpoint tpBump n l T := match T with
 	Uv => Uv |
-	El p => El (pBump n l p) |
-	Pi A B => Pi (fBump n l A) (fBump n (S l) B)
+	El t => El (ttBump n l t) |
+	Pi A B => Pi (tpBump n l A) (tpBump n (S l) B)
 end.
 
-Fixpoint fSubst F l b := match F with
-	Uv => Uv |
-	El p => El (pSubst p l b) |
-	Pi A B => Pi (fSubst A l b) (fSubst B (S l) b)
-end.
+Lemma ttBump_O l t : ttBump O l t = t.
+	induction t;simpl.
 
-Fixpoint tcBump n G := match G with
-	nil => nil |
-	F :: G => fBump n (length G) F :: tcBump n G
-end.
+	rewrite varBump_O.
+	reflexivity.
 
-Fixpoint tcSubst G b := match G with
-	nil => nil |
-	F :: G => fSubst F (length G) b :: tcSubst G b
-end.
-
-Lemma pBump_O l p : pBump O l p = p.
-	destruct p as (f,la).
-	simpl.
-	rewrite laBump_O.
-	unfold varBump.
-	simpl.
-	destruct (nat_compare f l);reflexivity.
+	rewrite IHt1.
+	rewrite IHt2.
+	reflexivity.
 Qed.
 
-Lemma pBump_Bump n1 n2 l1 l2 p : (l1 <= l2)->(pBump n2 (n1 + l2) (pBump n1 l1 p) = pBump n1 l1 (pBump n2 l2 p)).
+Lemma ttBump_Bump n1 n2 l1 l2 t : (l1 <= l2)->
+(ttBump n2 (n1 + l2) (ttBump n1 l1 t) = ttBump n1 l1 (ttBump n2 l2 t)).
 	intro.
-	destruct p as (f,la).
-	simpl.
+	induction t;simpl.
+
 	rewrite varBump_Bump with (1 := H).
-	rewrite laBump_Bump with (1 := H).
+	reflexivity.
+
+	rewrite IHt1.
+	rewrite IHt2.
 	reflexivity.
 Qed.
 
-Lemma pBumpDiv a b n l p : (n <= b)->(pBump a (l + n) (pBump b l p) = pBump (a + b) l p).
+Lemma ttBumpDiv a b n l t : (n <= b)->(ttBump a (l + n) (ttBump b l t) = ttBump (a + b) l t).
 	intro.
-	destruct p as (f,la).
-	simpl.
+	induction t;simpl.
+
 	rewrite varBumpDiv with (1 := H).
-	rewrite laBumpDiv with (1 := H).
+	reflexivity.
+
+	rewrite IHt1.
+	rewrite IHt2.
 	reflexivity.
 Qed.
 
-Lemma pBump_Subst n x p l b : pBump n (x + l) (pSubst p l b) = pSubst (pBump n (S x + l) p) l (varBump n x b).
-	destruct p as (f,la).
-	simpl.
-	change (S (x + l)) with (S x + l).
-	rewrite <- varBump_Subst.
-	rewrite <- laBump_Subst.
+Lemma tpBump_O T : forall l,tpBump O l T = T.
+	induction T;intro;simpl.
+
+	reflexivity.
+
+	rewrite ttBump_O.
+	reflexivity.
+
+	rewrite IHT1.
+	rewrite IHT2.
 	reflexivity.
 Qed.
 
-Lemma pSubst_Bump n p l1 l2 b : (l1 <= l2)->(pSubst (pBump n l1 p) (n + l2) b = pBump n l1 (pSubst p l2 b)).
-	intro.
-	destruct p as (f,la).
-	simpl.
-	rewrite varSubst_Bump with (1 := H).
-	rewrite laSubst_Bump with (1 := H).
-	reflexivity.
-Qed.
-
-Lemma pSubstDiv n p l1 l2 b : (l1 <= l2 <= l1 + n)->(pSubst (pBump (S n) l1 p) l2 b = pBump n l1 p).
-	intro.
-	destruct p as (f,la).
-	simpl.
-	rewrite varSubstDiv with (1 := H).
-	rewrite laSubstDiv with (1 := H).
-	reflexivity.
-Qed.
-
-Lemma pSubst_Subst x p l b1 b2 : pSubst (pSubst p l b2) (x + l) b1 =
-pSubst (pSubst p (S x + l) b1) l (varSubst x b1 b2).
-	destruct p as (f,la).
-	simpl.
-	change (S (x + l)) with (S x + l).
-	rewrite <- varSubst_Subst.
-	rewrite <- laSubst_Subst.
-	reflexivity.
-Qed.
-
-Lemma fBump_O F : forall l,fBump O l F = F.
-	induction F;intro;simpl.
+Lemma tpBump_Bump n1 n2 T : forall l1 l2,(l1 <= l2)->
+(tpBump n2 (n1 + l2) (tpBump n1 l1 T) = tpBump n1 l1 (tpBump n2 l2 T)).
+	induction T;intros;simpl.
 
 	reflexivity.
 
-	rewrite pBump_O.
-	reflexivity.
-
-	rewrite IHF1.
-	rewrite IHF2.
-	reflexivity.
-Qed.
-
-Lemma fBump_Bump n1 n2 F : forall l1 l2,(l1 <= l2)->
-(fBump n2 (n1 + l2) (fBump n1 l1 F) = fBump n1 l1 (fBump n2 l2 F)).
-	induction F;intros;simpl.
-
-	reflexivity.
-
-	rewrite pBump_Bump with (1 := H).
+	rewrite ttBump_Bump with (1 := H).
 	reflexivity.
 
 	rewrite plus_n_Sm.
-	rewrite IHF1 with (1 := H).
-	rewrite IHF2 with (1 := le_n_S _ _ H).
+	rewrite IHT1 with (1 := H).
+	rewrite IHT2 with (1 := le_n_S _ _ H).
 	reflexivity.
 Qed.
 
-Lemma fBumpDiv a b n F : (n <= b)->forall l,fBump a (l + n) (fBump b l F) = fBump (a + b) l F.
+Lemma tpBumpDiv a b n T : (n <= b)->forall l,tpBump a (l + n) (tpBump b l T) = tpBump (a + b) l T.
 	intro.
-	induction F;intro;simpl.
+	induction T;intro;simpl.
 
 	reflexivity.
 
-	rewrite pBumpDiv with (1 := H).
+	rewrite ttBumpDiv with (1 := H).
 	reflexivity.
 
 	change (S (l + n)) with (S l + n).
-	rewrite IHF1.
-	rewrite IHF2.
+	rewrite IHT1.
+	rewrite IHT2.
 	reflexivity.
 Qed.
 
-Lemma fBump_Subst n x F b : forall l,
-fBump n (x + l) (fSubst F l b) = fSubst (fBump n (S x + l) F) l (varBump n x b).
-	induction F;intro;simpl.
+Module Import TreeTermBump <: TERMBUMP.
 
-	reflexivity.
+Definition term := treeTerm.
 
-	change (S (x + l)) with (S x + l).
-	rewrite <- pBump_Subst.
-	reflexivity.
+Definition tmVar := var.
+Definition tmBump := ttBump.
 
-	change (S (x + l)) with (S x + l) at 2.
-	rewrite plus_n_Sm.
-	change (S (x + S l)) with (S x + S l).
-	rewrite <- IHF1.
-	rewrite <- IHF2.
+Lemma tmBump_Var n l i : tmBump n l (tmVar i) = tmVar (varBump n l i).
 	reflexivity.
 Qed.
 
-Lemma fSubst_Bump n F b : forall l1 l2,(l1 <= l2)->
-(fSubst (fBump n l1 F) (n + l2) b = fBump n l1 (fSubst F l2 b)).
-	induction F;intros;simpl.
+Definition tmBump_Bump := ttBump_Bump.
+Definition tmBumpDiv := ttBumpDiv.
 
-	reflexivity.
+End TreeTermBump.
 
-	rewrite pSubst_Bump with (1 := H).
-	reflexivity.
+Module Import TreeVarSubst := VarSubst TreeTermBump.
 
-	rewrite plus_n_Sm.
-	rewrite IHF1 with (1 := H).
-	rewrite IHF2 with (1 := le_n_S _ _ H).
-	reflexivity.
-Qed.
-
-Lemma fSubstDiv n F b : forall l1 l2,(l1 <= l2 <= l1 + n)->(fSubst (fBump (S n) l1 F) l2 b = fBump n l1 F).
-	induction F;intros;simpl.
-
-	reflexivity.
-
-	rewrite pSubstDiv with (1 := H).
-	reflexivity.
-
-	rewrite IHF1 with (1 := H).
-	rewrite IHF2.
-		reflexivity.
-	destruct H.
-	exact (conj (le_n_S _ _ H) (le_n_S _ _ H0)).
-Qed.
-
-Lemma fSubst_Subst x F b1 b2 : forall l,fSubst (fSubst F l b2) (x + l) b1 =
-fSubst (fSubst F (S x + l) b1) l (varSubst x b1 b2).
-	induction F;intros;simpl.
-
-	reflexivity.
-
-	change (S (x + l)) with (S x + l).
-	rewrite <- pSubst_Subst.
-	reflexivity.
-
-	change (S (x + l)) with (S x + l) at 2.
-	rewrite plus_n_Sm.
-	change (S (x + S l)) with (S x + S l).
-	rewrite <- IHF1.
-	rewrite <- IHF2.
-	reflexivity.
-Qed.
-
-Lemma tcBump_length n G : length (tcBump n G) = length G.
-	induction G;simpl.
-
-	reflexivity.
-
-	rewrite IHG.
-	reflexivity.
-Qed.
-
-Lemma tcBump_nth i n : forall G,(i < length G)->(nth i (tcBump n G) Uv = fBump n (length G - S i) (nth i G Uv)).
-	induction i;intro;(destruct G as [| F];intro;[destruct lt_n_O with (1 := H) |]);simpl.
-
-	rewrite <- minus_n_O.
-	reflexivity.
-
-	apply IHi.
-	apply lt_S_n with (1 := H).
-Qed.
-
-Lemma tcSubst_length G b : length (tcSubst G b) = length G.
-	induction G;simpl.
-
-	reflexivity.
-
-	rewrite IHG.
-	reflexivity.
-Qed.
-
-Lemma tcSubst_nth i b : forall G,(i < length G)->
-(nth i (tcSubst G b) Uv = fSubst (nth i G Uv) (length G - S i) b).
-	induction i;intro;(destruct G as [| F];intro;[destruct lt_n_O with (1 := H) |]);simpl.
-
-	rewrite <- minus_n_O.
-	reflexivity.
-
-	apply IHi.
-	apply lt_S_n with (1 := H).
-Qed.
-
-(* One-context typing rules. SimpParamGood is a "nested" inductive family. *)
-
-Inductive TreeFamGood PG G : treeFam->Type :=
-	tfGoodUv : TreeFamGood PG G Uv |
-	tfGoodEl f la : (f < length G)->
-		PG G (fBump (S f) O (nth f G Uv)) la Uv->
-		TreeFamGood PG G (El (f,la)) |
-	tfGoodPi A B : TreeFamGood PG G A->TreeFamGood PG (A :: G) B->
-		TreeFamGood PG G (Pi A B).
-
-Unset Elimination Schemes.
-Inductive SimpParamGood G F : list nat->treeFam->Set :=
-	spGoodNil : SimpParamGood G F nil F |
-	spGoodCons a la B : (a < length G)->
-		SimpParamGood G F la (Pi (fBump (S a) O (nth a G Uv)) B)->
-		SimpParamGood G F (a :: la) (fSubst B O a).
-Set Elimination Schemes.
-
-(* Mapping the PG in a TreeFamGood *)
-Section TFGMap.
-
-Variable A B : list treeFam->treeFam->list nat->treeFam->Type.
-Variable X : forall G F la T,A G F la T->B G F la T.
-
-Fixpoint tfGoodMap G F (HF:TreeFamGood A G F) : TreeFamGood B G F := match HF with
-	tfGoodUv => tfGoodUv _ _ |
-	tfGoodEl _ _ H HP => tfGoodEl _ _ _ _ H (X _ _ _ _ HP) |
-	tfGoodPi _ _ HA HB => tfGoodPi _ _ _ _ (tfGoodMap _ _ HA) (tfGoodMap _ _ HB)
+Fixpoint ttSubst l (b t:treeTerm) : treeTerm := match t with
+	var i => varSubst l b i |
+	apl f a => apl (ttSubst l b f) (ttSubst l b a)
 end.
 
-End TFGMap.
-Implicit Arguments tfGoodMap [A B G F].
-
-(* A (non-dependent) nested recursion principle for SimpParamGood *)
-Section SPGRect.
-
-Variable P : list treeFam->treeFam->list nat->treeFam->Type.
-
-Variable Pnil : forall G F,P G F nil F.
-Variable Pcons : forall G F a la B,(a < length G)->
-	P G F la (Pi (fBump (S a) O (nth a G Uv)) B)->
-	P G F (a :: la) (fSubst B O a).
-
-Fixpoint SimpParamGood_rect G F la T (Hla:SimpParamGood G F la T) : P G F la T := match Hla with
-	spGoodNil => Pnil _ _ |
-	spGoodCons _ _ _ H Hla => Pcons _ _ _ _ _ H (SimpParamGood_rect _ _ _ _ Hla)
+Fixpoint tpSubst l b T := match T with
+	Uv => Uv |
+	El t => El (ttSubst l b t) |
+	Pi A B => Pi (tpSubst l b A) (tpSubst (S l) b B)
 end.
 
-End SPGRect.
+Lemma ttBump_Subst n x l b t :
+ttBump n (x + l) (ttSubst l b t) = ttSubst l (ttBump n x b) (ttBump n (S x + l) t).
+	induction t;simpl.
 
-Definition SimpParamGood_ind (P:list treeFam->treeFam->list nat->treeFam->Prop) := SimpParamGood_rect P.
-Definition SimpParamGood_rec (P:list treeFam->treeFam->list nat->treeFam->Set) := SimpParamGood_rect P.
+	apply varBump_Subst.
 
-Definition TreeFamGoodPG := TreeFamGood SimpParamGood.
-
-Inductive TreeCtxGood : list treeFam->Set :=
-	tcGoodNil : TreeCtxGood nil |
-	tcGoodCons F G : TreeFamGoodPG G F->TreeCtxGood G->TreeCtxGood (F :: G).
-
-Lemma ctxProjGood i : forall G,TreeCtxGood G->TreeFamGoodPG (skipn (S i) G) (nth i G Uv).
-	induction i;intros;(destruct H;[simpl;apply tfGoodUv |]).
-
-	exact t.
-
-	exact (IHi _ H).
+	change (S (x + l)) with (S x + l).
+	rewrite <- IHt1.
+	rewrite <- IHt2.
+	reflexivity.
 Qed.
 
-Lemma tfGoodBumpNest GL X GR F : TreeFamGood (fun G F la T=>forall GR,(G = GR ++ GL)->
-	SimpParamGood (tcBump (length X) GR ++ X ++ GL) (fBump (length X) (length GR) F)
-		(laBump (length X) (length GR) la) (fBump (length X) (length GR) T))
-	(GR ++ GL) F->
-TreeFamGoodPG (tcBump (length X) GR ++ X ++ GL) (fBump (length X) (length GR) F).
-	set (P G F la T := forall GR,(G = GR ++ GL)->
-		SimpParamGood (tcBump (length X) GR ++ X ++ GL) (fBump (length X) (length GR) F)
-			(laBump (length X) (length GR) la) (fBump (length X) (length GR) T)).
+Lemma ttSubst_Bump n l1 l2 b t : (l1 <= l2)->
+(ttSubst (n + l2) b (ttBump n l1 t) = ttBump n l1 (ttSubst l2 b t)).
+	intro.
+	induction t;simpl.
+
+	apply varSubst_Bump with (1 := H).
+
+	rewrite IHt1.
+	rewrite IHt2.
+	reflexivity.
+Qed.
+
+Lemma ttSubstDiv n l1 l2 b t : (l1 <= l2 <= l1 + n)->(ttSubst l2 b (ttBump (S n) l1 t) = ttBump n l1 t).
+	intro.
+	induction t;simpl.
+
+	apply varSubstDiv with (1 := H).
+
+	rewrite IHt1.
+	rewrite IHt2.
+	reflexivity.
+Qed.
+
+Lemma tpBump_Subst n x b T : forall l,
+tpBump n (x + l) (tpSubst l b T) = tpSubst l (ttBump n x b) (tpBump n (S x + l) T).
+	induction T;intro;simpl.
+
+	reflexivity.
+
+	rewrite <- ttBump_Subst.
+	reflexivity.
+
+	rewrite <- IHT1.
+	rewrite plus_n_Sm.
+	rewrite <- IHT2.
+	reflexivity.
+Qed.
+
+Lemma tpSubst_Bump n b T : forall l1 l2,(l1 <= l2)->
+(tpSubst (n + l2) b (tpBump n l1 T) = tpBump n l1 (tpSubst l2 b T)).
+	induction T;intros;simpl.
+
+	reflexivity.
+
+	rewrite ttSubst_Bump with (1 := H).
+	reflexivity.
+
+	rewrite plus_n_Sm.
+	rewrite IHT1 with (1 := H).
+	rewrite IHT2 with (1 := le_n_S _ _ H).
+	reflexivity.
+Qed.
+
+Lemma tpSubstDiv n b T : forall l1 l2,(l1 <= l2 <= l1 + n)->(tpSubst l2 b (tpBump (S n) l1 T) = tpBump n l1 T).
+	induction T;intros;simpl.
+
+	reflexivity.
+
+	rewrite ttSubstDiv with (1 := H).
+	reflexivity.
+
+	rewrite IHT1 with (1 := H).
+	rewrite IHT2;[| destruct H;simpl;exact (conj (le_n_S _ _ H) (le_n_S _ _ H0))].
+	reflexivity.
+Qed.
+
+Module Import TreeTermSubst <: TERMSUBST.
+
+Module TermBump := TreeTermBump.
+Module VarSubst := TreeVarSubst.
+
+Definition tmSubst := ttSubst.
+
+Lemma tmSubst_Var l b i : tmSubst l b (tmVar i) = varSubst l b i.
+	reflexivity.
+Qed.
+
+Definition tmSubst_Bump := ttSubst_Bump.
+Definition tmSubstDiv := ttSubstDiv.
+
+End TreeTermSubst.
+
+Module Import TreeVarSubstSubst := VarSubstSubst TreeTermSubst.
+
+Lemma ttSubst_Subst x l b1 b2 t : ttSubst (x + l) b1 (ttSubst l b2 t) =
+ttSubst l (ttSubst x b1 b2) (ttSubst (S x + l) b1 t).
+	induction t;simpl.
+
+	apply varSubst_Subst.
+
+	change (S (x + l)) with (S x + l).
+	rewrite <- IHt1.
+	rewrite <- IHt2.
+	reflexivity.
+Qed.
+
+Lemma tpSubst_Subst x b1 b2 T : forall l,tpSubst (x + l) b1 (tpSubst l b2 T) =
+tpSubst l (ttSubst x b1 b2) (tpSubst (S x + l) b1 T).
+	induction T;intro;simpl.
+
+	reflexivity.
+
+	rewrite <- ttSubst_Subst.
+	reflexivity.
+
+	rewrite <- IHT1.
+	rewrite plus_n_Sm.
+	rewrite <- IHT2.
+	reflexivity.
+Qed.
+
+Module Import TreeTypes <: TYPES.
+
+Module TermBump := TreeTermBump.
+
+Definition type := treeType.
+
+Definition tyDf := Uv.
+Definition tyBump := tpBump.
+Definition tySubst := tpSubst.
+
+Definition tyBump_Bump := tpBump_Bump.
+Definition tyBumpDiv := tpBumpDiv.
+Definition tySubst_Bump := tpSubst_Bump.
+Definition tySubstDiv := tpSubstDiv.
+
+End TreeTypes.
+
+Module Import TreeVarOKBump := VarOKBump TreeTypes.
+
+Inductive TreeTermOK (G:list treeType) : treeTerm->treeType->Set :=
+	ttOKVar i (T:treeType) : VarOK G i T->TreeTermOK G (var i) T |
+	ttOKApl A B f a : TreeTermOK G f (Pi A B)->TreeTermOK G a A->
+		TreeTermOK G (apl f a) (tpSubst O a B).
+
+Inductive TreeTypeOK G : treeType->Set :=
+	tpOKUv : TreeTypeOK G Uv |
+	tpOKEl t : TreeTermOK G t Uv->TreeTypeOK G (El t) |
+	tpOKPi A B : TreeTypeOK G A->TreeTypeOK (A :: G) B->TreeTypeOK G (Pi A B).
+
+Lemma ttOKBump GL X GR t T : TreeTermOK (GR ++ GL) t T->
+TreeTermOK (ctxBump (length X) GR ++ X ++ GL) (ttBump (length X) (length GR) t) (tpBump (length X) (length GR) T).
 	remember (GR ++ GL) as G.
 	intro.
 	revert GR HeqG.
 	induction H;intros;simpl.
 
-	apply tfGoodUv.
+	apply ttOKVar.
+	apply varOKBump.
+	unfold type.
+	rewrite <- HeqG.
+	exact v.
 
-	subst P.
-	simpl in p.
-	pose proof (p _ HeqG).
-	clear p.
-	destruct (le_lt_dec (length GR) f).
-		subst G.
-		rewrite varBumpHi with (1 := le_not_lt _ _ l0).
-		apply tfGoodEl.
-			rewrite app_length.
-			rewrite tcBump_length.
-			rewrite app_length.
-			rewrite plus_assoc.
-			rewrite <- (plus_comm (length X)).
-			rewrite <- plus_assoc.
-			apply plus_lt_compat_l.
-			rewrite <- app_length.
-			exact l.
-		rewrite app_nth2;rewrite tcBump_length;[| apply le_trans with (1 := l0);apply le_plus_r].
-		rewrite <- le_plus_minus_assoc with (1 := l0).
-		rewrite app_nth2;[| apply le_plus_l].
-		rewrite minus_plus.
-		rewrite plus_n_Sm.
-		rewrite <- fBumpDiv with (1 := le_S _ _ l0).
-		simpl.
-		rewrite <- app_nth2 with (1 := l0).
-		exact H.
-
-		clear l.
-		subst G.
-		rewrite varBumpLo with (1 := l0).
-		apply tfGoodEl.
-			rewrite app_length.
-			rewrite tcBump_length.
-			apply le_trans with (1 := l0).
-			apply le_plus_l.
-		rewrite app_nth1;[| rewrite tcBump_length;exact l0].
-		rewrite tcBump_nth with (1 := l0).
-		rewrite <- fBump_Bump with (1 := le_O_n _).
-		rewrite <- le_plus_minus with (1 := l0).
-		rewrite <- app_nth1 with (l' := GL) (1 := l0).
-		exact H.
-
-	apply tfGoodPi.
-		exact (IHTreeFamGood1 _ HeqG).
-
-		apply (IHTreeFamGood2 (A :: GR)).
-		simpl.
-		rewrite <- HeqG.
-		reflexivity.
+	assert (IH1 := IHTreeTermOK1 _ HeqG).
+	assert (IH2 := IHTreeTermOK2 _ HeqG).
+	clear IHTreeTermOK1 IHTreeTermOK2.
+	simpl in IH1.
+	set (gr := length GR) at 3.
+	rewrite (plus_n_O gr).
+	subst gr.
+	rewrite tpBump_Subst.
+	rewrite <- plus_n_O.
+	apply ttOKApl with (1 := IH1) (2 := IH2).
 Qed.
 
-Lemma spGoodBump GL X GR F la T : SimpParamGood (GR ++ GL) F la T->
-SimpParamGood (tcBump (length X) GR ++ X ++ GL) (fBump (length X) (length GR) F)
-(laBump (length X) (length GR) la) (fBump (length X) (length GR) T).
+Lemma tpOKBump GL X GR T : TreeTypeOK (GR ++ GL) T->
+TreeTypeOK (ctxBump (length X) GR ++ X ++ GL) (tpBump (length X) (length GR) T).
 	remember (GR ++ GL) as G.
 	intro.
 	revert GR HeqG.
 	induction H;intros;simpl.
 
-	apply spGoodNil.
+	apply tpOKUv.
 
-	assert (IH := IHSimpParamGood _ HeqG).
-	clear IHSimpParamGood.
-	set (gr := length GR) at 4.
-	rewrite (plus_n_O gr).
-	subst gr.
-	rewrite fBump_Subst.
-	simpl.
-	rewrite <- plus_n_O.
-	destruct (le_lt_dec (length GR) a).
-		subst G.
-		rewrite varBumpHi with (1 := le_not_lt _ _ l).
-		assert (let a' := length X + a in
-		fBump (length X) (length GR) (fBump (S a) O (nth a (GR ++ GL) Uv)) =
-		fBump (S a') O (nth a' (tcBump (length X) GR ++ X ++ GL) Uv)).
-			simpl.
-			rewrite app_nth2 with (1 := l).
-			rewrite app_nth2;rewrite tcBump_length;[| apply le_trans with (1 := l);apply le_plus_r].
-			rewrite <- le_plus_minus_assoc with (1 := l).
-			rewrite app_nth2 with (1 := le_plus_l _ _).
-			rewrite minus_plus.
-			change (length GR) at 1 with (O + length GR).
-			rewrite fBumpDiv with (1 := le_S _ _ l).
-			rewrite <- plus_n_Sm.
-			reflexivity.
-		simpl in H0.
-		apply spGoodCons.
-			rewrite app_length.
-			rewrite tcBump_length.
-			rewrite app_length.
-			rewrite plus_assoc.
-			rewrite <- (plus_comm (length X)).
-			rewrite <- plus_assoc.
-			apply plus_lt_compat_l.
-			rewrite <- app_length.
-			exact H.
-		rewrite <- H0.
-		exact IH.
+	apply tpOKEl.
+	change Uv with (tpBump (length X) (length GR) Uv).
+	apply ttOKBump.
+	rewrite <- HeqG.
+	exact t0.
 
-		clear H.
-		subst G.
-		rewrite varBumpLo with (1 := l).
-		assert (fBump (length X) (length GR) (fBump (S a) O (nth a (GR ++ GL) Uv)) =
-		fBump (S a) O (nth a (tcBump (length X) GR ++ X ++ GL) Uv)).
-			rewrite app_nth1 with (1 := l).
-			rewrite app_nth1;[| rewrite tcBump_length;exact l].
-			rewrite tcBump_nth with (1 := l).
-			rewrite <- fBump_Bump with (1 := le_O_n _).
-			rewrite <- le_plus_minus with (1 := l).
-			reflexivity.
-		apply spGoodCons.
-			rewrite app_length.
-			rewrite tcBump_length.
-			apply le_trans with (1 := l).
-			apply le_plus_l.
-		rewrite <- H.
-		exact IH.
-Qed.
+	apply tpOKPi.
+		exact (IHTreeTypeOK1 _ HeqG).
 
-Lemma tfGoodBump GL X GR F : TreeFamGoodPG (GR ++ GL) F->
-TreeFamGoodPG (tcBump (length X) GR ++ X ++ GL) (fBump (length X) (length GR) F).
-	intro.
-	apply tfGoodBumpNest.
-	revert H.
-	apply tfGoodMap.
-	clear GR F.
-	intros.
-	apply spGoodBump.
-	rewrite <- H0.
-	exact H.
-Qed.
-
-Lemma tfGoodBump_O G X F : TreeFamGoodPG G F->TreeFamGoodPG (X ++ G) (fBump (length X) O F).
-	apply (tfGoodBump G X nil).
-Qed.
-
-Lemma tfGoodBump_unskip G n F : (n <= length G)->TreeFamGoodPG (skipn n G) F->TreeFamGoodPG G (fBump n O F).
-	intros.
-	rewrite <- (firstn_skipn n G).
-	set n at 3.
-	replace n0 with (length (firstn n G));subst n0.
-		apply tfGoodBump_O with (1 := H0).
-	rewrite firstn_length.
-	apply min_l with (1 := H).
-Qed.
-
-Lemma tfGoodSubstNest GL GR F b : (b < length GL)->let X := fBump (S b) O (nth b GL Uv) in
-TreeFamGood (fun G F la T=>forall GR,(G = GR ++ X :: GL)->
-	SimpParamGood (tcSubst GR b ++ GL) (fSubst F (length GR) b)
-		(laSubst la (length GR) b) (fSubst T (length GR) b))
-	(GR ++ X :: GL) F->
-TreeFamGoodPG (tcSubst GR b ++ GL) (fSubst F (length GR) b).
-	intros ? ?.
-	set (P G F la T := forall GR,(G = GR ++ X :: GL)->
-		SimpParamGood (tcSubst GR b ++ GL) (fSubst F (length GR) b)
-			(laSubst la (length GR) b) (fSubst T (length GR) b)).
-	remember (GR ++ X :: GL) as G.
-	intro.
-	revert GR HeqG.
-	induction H0;intros;simpl.
-
-	apply tfGoodUv.
-
-	subst P.
-	simpl in p.
-	pose proof (p _ HeqG).
-	clear p.
-	destruct (lt_eq_lt_dec f (length GR));[clear l;destruct s |].
-		rewrite varSubstLt with (1 := l).
-		subst G.
-		apply tfGoodEl.
-			rewrite app_length.
-			rewrite tcSubst_length.
-			apply le_trans with (1 := l).
-			apply le_plus_l.
-		rewrite app_nth1;[| rewrite tcSubst_length;exact l].
-		rewrite tcSubst_nth with (1 := l).
-		rewrite <- fSubst_Bump with (1 := le_O_n _).
-		rewrite <- le_plus_minus with (1 := l).
-		rewrite <- app_nth1 with (l' := X :: GL) (1 := l).
-		exact H0.
-
-		rewrite varSubstEq with (1 := e).
-		revert H0.
-		rewrite HeqG.
-		rewrite e.
-		clear G f HeqG e.
-		rewrite app_nth2 with (1 := le_n _).
-		rewrite minus_diag.
-		simpl.
-		intro.
-		apply tfGoodEl.
-			rewrite app_length.
-			rewrite tcSubst_length.
-			apply plus_lt_compat_l with (1 := H).
-		rewrite app_nth2;rewrite tcSubst_length;[| apply le_plus_l].
-		rewrite minus_plus.
-		rewrite plus_n_Sm.
-		rewrite <- fSubstDiv with (l2 := length GR) (b := b)
-			(1 := conj (le_O_n _) (le_plus_l _ _)).
-		change (S (length GR + S b)) with (S (length GR) + S b).
-		rewrite <- fBumpDiv with (1 := le_O_n _).
-		exact H0.
-
-		rewrite varSubstGt with (1 := l0).
-		revert l H0.
-		rewrite HeqG.
-		clear G HeqG.
-		destruct f.
-			destruct lt_n_O with (1 := l0).
-		rewrite app_length.
-		simpl.
-		rewrite <- plus_n_Sm.
-		intro.
-		rewrite app_nth2 with (1 := lt_le_weak _ _ l0).
-		pose proof (le_S_n _ _ l0).
-		pose proof (lt_S_n _ _ l).
-		clear l0 l.
-		rewrite <- minus_Sn_m with (1 := H0).
-		simpl.
-		intro.
-		apply tfGoodEl.
-			rewrite app_length.
-			rewrite tcSubst_length.
-			exact H1.
-		rewrite app_nth2;rewrite tcSubst_length;[| exact H0].
-		rewrite <- fSubstDiv with (l2 := length GR) (b := b)
-			(1 := conj (le_O_n _) (le_S _ _ H0)).
-		exact H2.
-
-	apply tfGoodPi.
-		exact (IHTreeFamGood1 _ HeqG).
-
-		apply (IHTreeFamGood2 (A :: GR)).
+		apply (IHTreeTypeOK2 (A :: GR)).
 		simpl.
 		rewrite <- HeqG.
 		reflexivity.
 Qed.
 
-Lemma spGoodSubst GL GR F la T b : (b < length GL)->
-	SimpParamGood (GR ++ fBump (S b) O (nth b GL Uv) :: GL) F la T->
-SimpParamGood (tcSubst GR b ++ GL) (fSubst F (length GR) b) (laSubst la (length GR) b) (fSubst T (length GR) b).
+Module Import TreeTypingBump <: TYPINGBUMP.
+
+Module Types := TreeTypes.
+Module VarSubst := TreeVarSubst.
+Module VarOKBump := TreeVarOKBump.
+
+Definition TermOK := TreeTermOK.
+Definition TypeOK := TreeTypeOK.
+
+Definition tmOKVar := ttOKVar.
+Definition tmOKBump := ttOKBump.
+
+End TreeTypingBump.
+
+Module Import TreeVarOKSubst := VarOKSubst TreeTypingBump.
+
+Lemma ttOKSubst GL b B GR t T : TreeTermOK GL b B->TreeTermOK (GR ++ B :: GL) t T->
+TreeTermOK (ctxSubst b GR ++ GL) (ttSubst (length GR) b t) (tpSubst (length GR) b T).
 	intro.
-	set (X := fBump (S b) O (nth b GL Uv)).
-	remember (GR ++ X :: GL) as G.
+	remember (GR ++ B :: GL) as G.
 	intro.
 	revert GR HeqG.
 	induction H0;intros;simpl.
 
-	apply spGoodNil.
+	apply varOKSubst with (1 := H).
+	unfold type.
+	rewrite <- HeqG.
+	exact v.
 
-	assert (IH := IHSimpParamGood _ HeqG).
-	clear IHSimpParamGood.
-	set (gr := length GR) at 4.
+	assert (IH1 := IHTreeTermOK1 _ HeqG).
+	assert (IH2 := IHTreeTermOK2 _ HeqG).
+	clear IHTreeTermOK1 IHTreeTermOK2.
+	simpl in IH1.
+	set (gr := length GR) at 3.
 	rewrite (plus_n_O gr).
 	subst gr.
-	rewrite fSubst_Subst.
-	simpl.
+	rewrite tpSubst_Subst.
 	rewrite <- plus_n_O.
-	destruct (lt_eq_lt_dec a (length GR));[clear H0;destruct s |].
-		rewrite varSubstLt with (1 := l).
-		subst G.
-		assert (fSubst (fBump (S a) O (nth a (GR ++ X :: GL) Uv)) (length GR) b =
-		fBump (S a) O (nth a (tcSubst GR b ++ GL) Uv)).
-			rewrite app_nth1 with (1 := l).
-			rewrite app_nth1;[| rewrite tcSubst_length;exact l].
-			rewrite tcSubst_nth with (1 := l).
-			rewrite <- fSubst_Bump with (1 := le_O_n _).
-			rewrite <- le_plus_minus with (1 := l).
-			reflexivity.
-		apply spGoodCons.
-			rewrite app_length.
-			rewrite tcSubst_length.
-			apply le_trans with (1 := l).
-			apply le_plus_l.
-		rewrite <- H0.
-		exact IH.
+	apply ttOKApl with (1 := IH1) (2 := IH2).
+Qed.
 
-		rewrite varSubstEq with (1 := e).
-		subst G.
-		assert (let a' := length GR + b in
-		fSubst (fBump (S a) O (nth a (GR ++ X :: GL) Uv)) (length GR) b =
-		fBump (S a') O (nth a' (tcSubst GR b ++ GL) Uv)).
-			rewrite e.
-			simpl.
-			rewrite app_nth2 with (1 := le_n _).
-			rewrite minus_diag.
-			simpl.
-			rewrite app_nth2;rewrite tcSubst_length;[| apply le_plus_l].
-			rewrite minus_plus.
-			rewrite fSubstDiv with (1 := conj (le_O_n (length GR)) (le_n _)).
-			rewrite plus_n_Sm.
-			rewrite <- fBumpDiv with (1 := le_O_n _).
-			simpl.
-			fold X.
-			reflexivity.
-		simpl in H0.
-		apply spGoodCons.
-			rewrite app_length.
-			rewrite tcSubst_length.
-			apply plus_lt_compat_l with (1 := H).
-		rewrite <- H0.
-		exact IH.
+Lemma tpOKSubst GL b B GR T : TreeTermOK GL b B->TreeTypeOK (GR ++ B :: GL) T->
+TreeTypeOK (ctxSubst b GR ++ GL) (tpSubst (length GR) b T).
+	intro.
+	remember (GR ++ B :: GL) as G.
+	intro.
+	revert GR HeqG.
+	induction H0;intros;simpl.
 
-		rewrite varSubstGt with (1 := l).
-		subst G.
-		revert H0 IH.
-		destruct a.
-			destruct lt_n_O with (1 := l).
-		rewrite app_length.
+	apply tpOKUv.
+
+	apply tpOKEl.
+	change Uv with (tpSubst (length GR) b Uv).
+	apply ttOKSubst with (1 := H).
+	rewrite <- HeqG.
+	exact t0.
+
+	apply tpOKPi.
+		exact (IHTreeTypeOK1 _ HeqG).
+
+		apply (IHTreeTypeOK2 (A :: GR)).
 		simpl.
-		rewrite <- plus_n_Sm.
-		intro.
-		rewrite app_nth2 with (1 := lt_le_weak _ _ l).
-		pose proof (le_S_n _ _ l).
-		pose proof (lt_S_n _ _ H0).
-		clear l H0.
-		rewrite <- minus_Sn_m with (1 := H1).
-		simpl.
-		rewrite fSubstDiv with (1 := conj (le_O_n _) (le_S _ _ H1)).
-		intros.
-		assert (nth (a - length GR) GL Uv =
-		nth a (tcSubst GR b ++ GL) Uv).
-			rewrite app_nth2;rewrite tcSubst_length;[| exact H1].
-			reflexivity.
-		apply spGoodCons.
-			rewrite app_length.
-			rewrite tcSubst_length.
-			exact H2.
-		rewrite <- H0.
-		exact IH.
-Qed.
-
-Lemma tfGoodSubst GL GR F b : (b < length GL)->TreeFamGoodPG (GR ++ fBump (S b) O (nth b GL Uv) :: GL) F->
-TreeFamGoodPG (tcSubst GR b ++ GL) (fSubst F (length GR) b).
-	intros.
-	apply tfGoodSubstNest with (1 := H).
-	revert H0.
-	apply tfGoodMap.
-	clear GR F.
-	intros.
-	apply spGoodSubst with (1 := H).
-	rewrite <- H1.
-	exact H0.
-Qed.
-
-Lemma tfGoodSubst_O G F b : (b < length G)->TreeFamGoodPG (fBump (S b) O (nth b G Uv) :: G) F->
-TreeFamGoodPG G (fSubst F O b).
-	apply (tfGoodSubst G nil).
-Qed.
-
-(* Conversion from two-context to one-context language *)
-
-Definition spTree l (p:_ * _) := let (f,la) := p in El (l + f,la).
-
-Fixpoint sfTree l (F:simpFam) := match F with
-	nil => Uv |
-	p :: F => Pi (spTree l p) (sfTree (S l) F)
-end.
-
-Definition sfcTree := map (sfTree O).
-
-Fixpoint spcTree G := match G with
-	nil => nil |
-	p :: G => spTree (length G) p :: spcTree G
-end.
-
-Lemma spcTree_length G : length (spcTree G) = length G.
-	induction G;simpl.
-
-	reflexivity.
-
-	rewrite IHG.
-	reflexivity.
-Qed.
-
-Lemma spcTree_nth a : forall G,(a < length G)->
-(nth a (spcTree G) Uv = spTree (length G - S a) (nth a G (O,nil))).
-	induction a;intro;(destruct G;intro;[destruct lt_n_O with (1 := H) |]);simpl.
-
-	rewrite <- minus_n_O.
-	reflexivity.
-
-	exact (IHa _ (lt_S_n _ _ H)).
-Qed.
-
-Lemma spTree_BumpG n l1 l2 p : (l1 <= l2)->(spTree (l2 + n) (pBumpG n l1 p) = fBump n l1 (spTree l2 p)).
-	intro.
-	destruct p as (f,la).
-	simpl.
-	rewrite varBumpHi;[| apply le_not_lt;apply le_trans with (1 := H);apply le_plus_l].
-	rewrite plus_assoc.
-	rewrite <- (plus_comm l2).
-	reflexivity.
-Qed.
-
-Lemma sfTree_BumpG n F : forall l1 l2,(l1 <= l2)->(sfTree (l2 + n) (fBumpG n l1 F) = fBump n l1 (sfTree l2 F)).
-	induction F;intros;simpl.
-
-	reflexivity.
-
-	rewrite spTree_BumpG with (1 := H).
-	change (S (l2 + n)) with (S l2 + n).
-	rewrite (IHF _ _ (le_n_S _ _ H)).
-	reflexivity.
-Qed.
-
-Lemma sfTree_BumpDG a b F : forall l,(fBumpG 1 l F = F)->
-(sfTree (l + a) (fBumpD b F) = fBump (a + b) l (sfTree l F)).
-	induction F as [| p].
-
-	simpl.
-	intros.
-	reflexivity.
-
-	intro.
-	destruct p as (f,la).
-	simpl.
-	intro.
-	replace (varBump (a + b) l (l + f)) with (l + a + (b + f));
-	[|
-		rewrite plus_assoc;
-		rewrite <- (plus_assoc l);
-		rewrite <- (plus_comm (a + b));
-		rewrite <- plus_assoc;
-		unfold varBump;
-		(destruct (nat_compare_spec (l + f) l);try reflexivity);
-		destruct (lt_n_O f);
-		apply plus_lt_reg_l with l;
-		rewrite <- plus_n_O;
-		exact H0
-	].
-	replace (laBump (a + b) l la) with la;
-	[|
-		symmetry;
-		apply laFreeBump;
-		change la at 2 with (snd (hd (O,nil) ((f,la) :: F)));
-		rewrite <- H;
-		simpl;
-		reflexivity
-	].
-	rewrite <- IHF.
+		rewrite <- HeqG.
 		reflexivity.
-	change F at 2 with (tl ((f,la) :: F)).
-	rewrite <- H.
-	simpl.
-	reflexivity.
-Qed.
-
-Lemma spTree_SubstG p l1 l2 b : (l1 <= l2)->(spTree l2 (pSubstG p l1 b) = fSubst (spTree (S l2) p) l1 b).
-	intro.
-	destruct p as (f,la).
-	simpl.
-	rewrite varSubstGt.
-		simpl.
-		reflexivity.
-	apply le_n_S.
-	apply le_trans with (1 := H).
-	apply le_plus_l.
-Qed.
-
-Lemma sfTree_SubstG F b : forall l1 l2,(l1 <= l2)->(sfTree l2 (fSubstG F l1 b) = fSubst (sfTree (S l2) F) l1 b).
-	induction F;intros;simpl.
-
-	reflexivity.
-
-	rewrite <- spTree_SubstG with (1 := H).
-	rewrite <- (IHF _ _ (le_n_S _ _ H)).
-	reflexivity.
-Qed.
-
-Lemma spOKGood D G F la T : let G' := spcTree G ++ sfcTree D in
-	TreeFamGoodPG G' (sfTree (length G) F)->
-	SimpParamOK G F la T->
-SimpParamGood G' (sfTree (length G) F) la (sfTree (length G) T).
-	simpl.
-	intros.
-	induction H0.
-
-	apply spGoodNil.
-
-	simpl in IHSimpParamOK.
-	rewrite sfTree_SubstG with (1 := le_O_n _).
-	assert (spTree (length G) (pBumpG (S a) O (nth a G (O,nil))) =
-	fBump (S a) O (nth a (spcTree G ++ sfcTree D) Uv)).
-		rewrite app_nth1;[| rewrite spcTree_length;exact l].
-		rewrite spcTree_nth with (1 := l).
-		rewrite <- spTree_BumpG with (1 := le_O_n _).
-		rewrite <- plus_comm.
-		rewrite <- le_plus_minus with (1 := l).
-		reflexivity.
-	assert (a < length (spcTree G ++ sfcTree D)).
-		rewrite app_length.
-		rewrite spcTree_length.
-		apply le_trans with (1 := l).
-		apply le_plus_l.
-	apply spGoodCons with (1 := H2).
-	rewrite <- H1.
-	exact IHSimpParamOK.
-Qed.
-
-Lemma sfOKGood D G T : SimpFCtxOK D->SimpFamOK D G T->let G' := spcTree G ++ sfcTree D in TreeCtxGood G'->
-TreeFamGoodPG G' (sfTree (length G) T).
-	intros HD ?.
-	simpl.
-	induction H;intro.
-
-	simpl.
-	apply tfGoodUv.
-
-	simpl in IHSimpFamOK |- *.
-	assert (TreeFamGoodPG (spcTree G ++ sfcTree D) (El (length G + f,la))).
-		assert (length G + f < length (spcTree G ++ sfcTree D)).
-			rewrite app_length.
-			rewrite spcTree_length.
-			apply plus_lt_compat_l.
-			unfold sfcTree.
-			rewrite map_length.
-			exact l.
-		apply tfGoodEl with (1 := H1).
-		assert (sfTree (length G) (fBumpD (S f) (nth f D nil)) =
-		fBump (S (length G + f)) O (nth (length G + f) (spcTree G ++ sfcTree D) Uv)).
-			rewrite plus_n_Sm.
-			rewrite app_nth2;rewrite spcTree_length;[| apply le_plus_l].
-			rewrite minus_plus.
-			unfold sfcTree.
-			change Uv with (sfTree O nil).
-			rewrite map_nth.
-			apply sfTree_BumpDG with (l := O).
-			pose proof (fctxProjOK _ _ HD l).
-			apply sfOKFree with (1 := H2).
-		refine (let H := spOKGood D _ _ _ _ _ s in _).
-			rewrite H2.
-			apply tfGoodBump_unskip with (1 := H1).
-			apply ctxProjGood with (1 := H0).
-		simpl in H3.
-		rewrite <- H2.
-		exact H3.
-	refine (let H := IHSimpFamOK _ in _).
-		apply tcGoodCons with (1 := H1) (2 := H0).
-	apply tfGoodPi with (1 := H1) (2 := H2).
 Qed.
