trunk/DepTyping.v
@@ -1,0 +1,232 @@
+Require Import List.
+
+Require Import Utils.
+Require Import Substitutions.
+
+Require Import Le Lt.
+Require Import Plus Minus.
+Require Import Compare_dec.
+
+Module Type TYPES.
+
+Declare Module Import TermBump : TERMBUMP.
+
+Parameter type : Type.
+
+Parameter tyDf : type.
+Parameter tyBump : forall (n l:nat) (T:type),type.
+Parameter tySubst : forall (l:nat) (b:term) (T:type),type.
+
+Axiom tyBump_Bump : forall n1 n2 T l1 l2,(l1 <= l2)->
+(tyBump n2 (n1 + l2) (tyBump n1 l1 T) = tyBump n1 l1 (tyBump n2 l2 T)).
+
+Axiom tyBumpDiv : forall a b n T,(n <= b)->forall l,tyBump a (l + n) (tyBump b l T) = tyBump (a + b) l T.
+
+Axiom tySubst_Bump : forall n b T l1 l2,(l1 <= l2)->
+(tySubst (n + l2) b (tyBump n l1 T) = tyBump n l1 (tySubst l2 b T)).
+
+Axiom tySubstDiv : forall n b T l1 l2,(l1 <= l2 <= l1 + n)->(tySubst l2 b (tyBump (S n) l1 T) = tyBump n l1 T).
+
+End TYPES.
+
+Module VarOKBump (Import Types : TYPES).
+
+Import VarBump.
+Import TermBump.
+
+Fixpoint ctxBump n G := match G with
+	nil => nil |
+	T :: G => tyBump n (length G) T :: ctxBump n G
+end.
+
+Fixpoint ctxSubst b G := match G with
+	nil => nil |
+	T :: G => tySubst (length G) b T :: ctxSubst b G
+end.
+
+Lemma ctxBump_length n G : length (ctxBump n G) = length G.
+	induction G;simpl.
+
+	reflexivity.
+
+	rewrite IHG.
+	reflexivity.
+Qed.
+
+Lemma ctxBump_nth i n : forall G,(i < length G)->(nth i (ctxBump n G) tyDf = tyBump n (length G - S i) (nth i G tyDf)).
+	induction i;intro;(destruct G as [| T];intro;[destruct lt_n_O with (1 := H) |]);simpl.
+
+	rewrite <- minus_n_O.
+	reflexivity.
+
+	apply IHi.
+	apply lt_S_n with (1 := H).
+Qed.
+
+Lemma ctxSubst_length b G : length (ctxSubst b G) = length G.
+	induction G;simpl.
+
+	reflexivity.
+
+	rewrite IHG.
+	reflexivity.
+Qed.
+
+Lemma ctxSubst_nth i b : forall G,(i < length G)->(nth i (ctxSubst b G) tyDf = tySubst (length G - S i) b (nth i G tyDf)).
+	induction i;intro;(destruct G as [| T];intro;[destruct lt_n_O with (1 := H) |]);simpl.
+
+	rewrite <- minus_n_O.
+	reflexivity.
+
+	apply IHi.
+	apply lt_S_n with (1 := H).
+Qed.
+
+Inductive VarOK G i : type->Set := mkVarOK : (i < length G)->VarOK G i (tyBump (S i) O (nth i G tyDf)).
+
+Lemma varOKBump GL X GR i T : VarOK (GR ++ GL) i T->
+VarOK (ctxBump (length X) GR ++ X ++ GL) (varBump (length X) (length GR) i) (tyBump (length X) (length GR) T).
+	intro.
+	destruct H.
+	destruct (le_lt_dec (length GR) i).
+
+	rewrite varBumpHi with (1 := le_not_lt _ _ l0).
+	assert (let i' := length X + i in
+	tyBump (length X) (length GR) (tyBump (S i) O (nth i (GR ++ GL) tyDf)) =
+	tyBump (S i') O (nth i' (ctxBump (length X) GR ++ X ++ GL) tyDf)).
+		simpl.
+		rewrite app_nth2 with (1 := l0).
+		rewrite app_nth2;rewrite ctxBump_length;[| apply le_trans with (1 := l0);apply le_plus_r].
+		rewrite <- le_plus_minus_assoc with (1 := l0).
+		rewrite app_nth2 with (1 := le_plus_l _ _).
+		rewrite minus_plus.
+		change (length GR) at 1 with (O + length GR).
+		rewrite tyBumpDiv with (1 := le_S _ _ l0).
+		rewrite plus_n_Sm.
+		reflexivity.
+	simpl in H.
+	rewrite H.
+	apply mkVarOK.
+	rewrite app_length.
+	rewrite ctxBump_length.
+	rewrite app_length.
+	rewrite plus_assoc.
+	rewrite <- (plus_comm (length X)).
+	rewrite <- plus_assoc.
+	apply plus_lt_compat_l.
+	rewrite <- app_length.
+	exact l.
+
+	rewrite varBumpLo with (1 := l0).
+	assert (tyBump (length X) (length GR) (tyBump (S i) O (nth i (GR ++ GL) tyDf)) =
+	tyBump (S i) O (nth i (ctxBump (length X) GR ++ X ++ GL) tyDf)).
+		rewrite app_nth1 with (1 := l0).
+		rewrite app_nth1;[| rewrite ctxBump_length;exact l0].
+		rewrite ctxBump_nth with (1 := l0).
+		rewrite <- tyBump_Bump with (1 := le_O_n _).
+		rewrite <- le_plus_minus with (1 := l0).
+		reflexivity.
+	rewrite H.
+	apply mkVarOK.
+	rewrite app_length.
+	rewrite ctxBump_length.
+	apply le_plus_trans with (1 := l0).
+Qed.
+
+End VarOKBump.
+
+Module Type TYPINGBUMP.
+
+Declare Module Import Types : TYPES.
+Import TermBump.
+
+Module VarSubst := VarSubst TermBump.
+Module Import VarOKBump := VarOKBump Types.
+
+Parameter TermOK : forall (G:list type) (t:term) (T:type),Type.
+Parameter TypeOK : forall (G:list type) (T:type),Type.
+
+Axiom tmOKVar : forall G i T,VarOK G i T->TermOK G (tmVar i) T.
+
+Axiom tmOKBump : forall GL X GR t T,TermOK (GR ++ GL) t T->
+TermOK (ctxBump (length X) GR ++ X ++ GL) (tmBump (length X) (length GR) t) (tyBump (length X) (length GR) T).
+
+End TYPINGBUMP.
+
+Module VarOKSubst (Import TypingBump : TYPINGBUMP).
+
+Import Types VarSubst VarOKBump.
+Import TermBump.
+
+Inductive CtxOK : list type->Type :=
+	ctxOKNil : CtxOK nil |
+	ctxOKCons G T : CtxOK G->TypeOK G T->CtxOK (T :: G).
+
+Lemma ctxProjOK i : forall G,CtxOK G->(i < length G)->TypeOK (skipn (S i) G) (nth i G tyDf).
+	induction i;intros;(destruct X;[destruct lt_n_O with (1 := H) |]).
+
+	exact t.
+
+	exact (IHi _ X (le_S_n _ _ H)).
+Qed.
+
+Lemma varOKSubst GL b B GR i T : TermOK GL b B->VarOK (GR ++ B :: GL) i T->
+TermOK (ctxSubst b GR ++ GL) (varSubst (length GR) b i) (tySubst (length GR) b T).
+	intros Hb Hi.
+	destruct Hi.
+	destruct (lt_eq_lt_dec i (length GR));[clear l;destruct s |].
+
+	rewrite varSubstLt with (1 := l).
+	assert (tySubst (length GR) b (tyBump (S i) O (nth i (GR ++ B :: GL) tyDf)) =
+	tyBump (S i) O (nth i (ctxSubst b GR ++ GL) tyDf)).
+		rewrite app_nth1 with (1 := l).
+		rewrite app_nth1;[| rewrite ctxSubst_length;exact l].
+		rewrite ctxSubst_nth with (1 := l).
+		rewrite <- tySubst_Bump with (1 := le_O_n _).
+		rewrite <- le_plus_minus with (1 := l).
+		reflexivity.
+	rewrite H.
+	apply tmOKVar.
+	apply mkVarOK.
+	rewrite app_length.
+	rewrite ctxSubst_length.
+	apply le_plus_trans with (1 := l).
+
+	rewrite varSubstEq with (1 := e).
+	subst i.
+	rewrite app_nth2 with (1 := le_n _).
+	rewrite minus_diag.
+	simpl.
+	rewrite tySubstDiv with (1 := conj (le_O_n _) (le_n (length GR))).
+	change (ctxSubst b GR ++ GL) with (ctxBump (length GR) nil ++ ctxSubst b GR ++ GL).
+	rewrite <- (ctxSubst_length b GR).
+	apply tmOKBump with (1 := Hb).
+
+	rewrite varSubstGt with (1 := l0).
+	revert l.
+	destruct i.
+		destruct lt_n_O with (1 := l0).
+	rewrite app_length.
+	simpl.
+	rewrite <- plus_n_Sm.
+	intro.
+	rewrite app_nth2 with (1 := lt_le_weak _ _ l0).
+	assert (Hlo := le_S_n _ _ l0).
+	assert (Hhi := lt_S_n _ _ l).
+	clear l0 l.
+	rewrite <- minus_Sn_m with (1 := Hlo).
+	simpl.
+	rewrite tySubstDiv with (1 := conj (le_O_n _) (le_S _ _ Hlo)).
+	assert (nth (i - length GR) GL tyDf =
+	nth i (ctxSubst b GR ++ GL) tyDf).
+		rewrite app_nth2;rewrite ctxSubst_length;[| exact Hlo].
+		reflexivity.
+	rewrite H.
+	apply tmOKVar.
+	apply mkVarOK.
+	rewrite app_length.
+	rewrite ctxSubst_length.
+	exact Hhi.
+Qed.
+
+End VarOKSubst.
