trunk/SimpToTree.v
@@ -1,0 +1,217 @@
+Require Import List.
+
+Require Import SimpSyntax.
+Require Import TreeSyntax.
+
+Require Import Le Lt.
+Require Import Plus Minus.
+Require Import Compare_dec.
+
+Require Import Utils.
+Require Import Substitutions.
+
+Import VarBump.
+Import TreeTermBump.
+Import TreeVarSubst.
+Import TreeVarOKBump.
+Import TreeVarOKSubst.
+
+Fixpoint laTree l f la := match la with
+	nil => var (l + f) |
+	a :: la => apl (laTree l f la) (var a)
+end.
+
+Definition spTree l (p:_ * _) := let (f,la) := p in El (laTree l f la).
+
+Fixpoint sfTree l (F:simpFam) := match F with
+	nil => Uv |
+	p :: F => Pi (spTree l p) (sfTree (S l) F)
+end.
+
+Definition sfcTree := map (sfTree O).
+
+Fixpoint spcTree G := match G with
+	nil => nil |
+	p :: G => spTree (length G) p :: spcTree G
+end.
+
+Lemma laTreeChLvl l f la : laTree l f la = laTree O (l + f) la.
+	induction la;simpl.
+
+	reflexivity.
+
+	rewrite <- IHla.
+	reflexivity.
+Qed.
+
+Lemma spcTree_length G : length (spcTree G) = length G.
+	induction G;simpl.
+
+	reflexivity.
+
+	rewrite IHG.
+	reflexivity.
+Qed.
+
+Lemma spcTree_nth a : forall G,(a < length G)->
+(nth a (spcTree G) Uv = spTree (length G - S a) (nth a G (O,nil))).
+	induction a;intro;(destruct G;intro;[destruct lt_n_O with (1 := H) |]);simpl.
+
+	rewrite <- minus_n_O.
+	reflexivity.
+
+	exact (IHa _ (lt_S_n _ _ H)).
+Qed.
+
+Lemma laTree_BumpG n l1 l2 f la : (l1 <= l2)->(laTree (l2 + n) f (laBump n l1 la) = ttBump n l1 (laTree l2 f la)).
+	intro.
+	induction la;simpl.
+
+	rewrite varBumpHi;[| apply le_not_lt;apply le_plus_trans with (1 := H)].
+	rewrite plus_assoc.
+	rewrite <- (plus_comm n).
+	reflexivity.
+
+	rewrite IHla.
+	reflexivity.
+Qed.
+
+Lemma spTree_BumpG n l1 l2 p : (l1 <= l2)->(spTree (l2 + n) (pBumpG n l1 p) = tpBump n l1 (spTree l2 p)).
+	intro.
+	destruct p as (f,la).
+	simpl.
+	rewrite laTree_BumpG with (1 := H).
+	reflexivity.
+Qed.
+
+Lemma sfTree_BumpG n F : forall l1 l2,(l1 <= l2)->(sfTree (l2 + n) (fBumpG n l1 F) = tpBump n l1 (sfTree l2 F)).
+	induction F;intros;simpl.
+
+	reflexivity.
+
+	rewrite spTree_BumpG with (1 := H).
+	change (S (l2 + n)) with (S l2 + n).
+	rewrite (IHF _ _ (le_n_S _ _ H)).
+	reflexivity.
+Qed.
+
+Lemma sfTree_BumpDG a b F : forall l,(fBumpG 1 l F = F)->
+(sfTree (l + a) (fBumpD b F) = tpBump (a + b) l (sfTree l F)).
+	induction F as [| p].
+
+	simpl.
+	intros.
+	reflexivity.
+
+	intro.
+	destruct p as (f,la).
+	simpl.
+	intro.
+	rewrite <- laTree_BumpG with (1 := le_n _).
+	rewrite (laTreeChLvl _ f).
+	rewrite plus_assoc.
+	rewrite <- plus_assoc.
+	rewrite <- laTreeChLvl.
+	pose proof (ap (fun F=>snd (hd (f,la) F)) H).
+	pose proof (ap (@tl _) H).
+	simpl in H0,H1.
+	clear H.
+	rewrite laFreeBump with (1 := H0).
+	rewrite <- (IHF _ H1).
+	reflexivity.
+Qed.
+
+Lemma var_simpVarSubst l b i : var (SimpSubst.varSubst l b i) = varSubst l (var b) i.
+	unfold SimpSubst.varSubst.
+	unfold varSubst.
+	destruct (nat_compare i l);[simpl;rewrite varBumpHi with (1 := lt_n_O _) | |];reflexivity.
+Qed.
+
+Lemma laTree_SubstG f la l1 l2 b : (l1 <= l2)->(laTree l2 f (laSubst la l1 b) = ttSubst l1 (var b) (laTree (S l2) f la)).
+	intro.
+	induction la;simpl.
+
+	rewrite varSubstGt;[| apply le_n_S;apply le_plus_trans with (1 := H)].
+	exact (eq_refl (var (l2 + f))).
+
+	rewrite <- IHla.
+	rewrite var_simpVarSubst.
+	reflexivity.
+Qed.
+
+Lemma spTree_SubstG p l1 l2 b : (l1 <= l2)->(spTree l2 (pSubstG p l1 b) = tpSubst l1 (var b) (spTree (S l2) p)).
+	intro.
+	destruct p as (f,la).
+	simpl.
+	rewrite <- laTree_SubstG with (1 := H).
+	reflexivity.
+Qed.
+
+Lemma sfTree_SubstG F b : forall l1 l2,(l1 <= l2)->(sfTree l2 (fSubstG F l1 b) = tpSubst l1 (var b) (sfTree (S l2) F)).
+	induction F;intros;simpl.
+
+	reflexivity.
+
+	rewrite <- spTree_SubstG with (1 := H).
+	rewrite <- (IHF _ _ (le_n_S _ _ H)).
+	reflexivity.
+Qed.
+
+Lemma spOKTree D G F f la T : SimpParamOK G F la T->let G' := spcTree G ++ sfcTree D in
+VarOK G' (length G + f) (sfTree (length G) F)->TreeTermOK G' (laTree (length G) f la) (sfTree (length G) T).
+	simpl.
+	intros Hla Hf.
+	induction Hla;simpl.
+
+	apply ttOKVar with (1 := Hf).
+
+	rewrite sfTree_SubstG with (1 := le_O_n _).
+	apply ttOKApl with (1 := IHHla).
+	apply ttOKVar.
+	rewrite le_plus_minus with (1 := l).
+	rewrite <- plus_comm.
+	rewrite spTree_BumpG with (1 := le_O_n _).
+	rewrite <- spcTree_nth with (1 := l).
+	assert (a < length (spcTree G)).
+		rewrite spcTree_length.
+		exact l.
+	rewrite <- app_nth1 with (l' := sfcTree D) (1 := H).
+	apply mkVarOK.
+	rewrite app_length.
+	apply le_plus_trans with (1 := H).
+Qed.
+
+Lemma sfOKTree D G T : SimpFCtxOK D->SimpFamOK D G T->let G' := spcTree G ++ sfcTree D in
+CtxOK G'->TreeTypeOK G' (sfTree (length G) T).
+	intros HD ?.
+	simpl.
+	induction H;intro.
+
+	simpl.
+	apply tpOKUv.
+
+	simpl in IHSimpFamOK |- *.
+	assert (TreeTypeOK (spcTree G ++ sfcTree D) (El (laTree (length G) f la))).
+		apply tpOKEl.
+		apply spOKTree with (1 := s).
+		change (length G) with (O + length G) at 2.
+		rewrite sfTree_BumpDG with (1 := sfOKFree _ _ _ (fctxProjOK _ _ HD l)).
+		simpl.
+		rewrite <- plus_n_Sm.
+		rewrite <- map_nth.
+		fold sfcTree.
+		simpl.
+		set (f' := f) at 3.
+		replace f' with (length G + f - length (spcTree G));subst f';[| rewrite spcTree_length;apply minus_plus].
+		rewrite <- app_nth2 with (l := spcTree G);[| rewrite spcTree_length;apply le_plus_l].
+		apply mkVarOK.
+		rewrite app_length.
+		rewrite spcTree_length.
+		apply plus_lt_compat_l.
+		unfold sfcTree.
+		rewrite map_length.
+		exact l.
+	refine (let H := IHSimpFamOK _ in _).
+		apply ctxOKCons with (1 := X) (2 := H0).
+	apply tpOKPi with (1 := H0) (2 := H1).
+Qed.
